BLS/bls-full-MODEL-AUTO.ec
@@ -1,14 +1,18 @@
 prover alt-ergo, z3, cvc3.
 
 type G_1.
+type G_2.
 type G_T.
 type message.
 
 cnst g_1_i : G_1.
+cnst g_2_i : G_2.
 cnst g_T_i : G_T.
-cnst g_1 : G_1.
+cnst g_1 : G_2.
+cnst g_2 : G_1.
 cnst g_T : G_T.
 cnst q_1 : int.
+cnst q_2 : int.
 cnst q_T : int.
 
 cnst q : int.
@@ -16,15 +20,18 @@ cnst q : int.
 cnst limit_Hash : int.
 
 op [*] : (G_1, G_1) -> G_1 as G_1_mul.
+op [*] : (G_2, G_2) -> G_2 as G_2_mul.
 op [^] : (G_1, int) -> G_1 as G_1_pow.
+op [^] : (G_2, int) -> G_2 as G_2_pow.
 
 op [*] : (G_T, G_T) -> G_T as G_T_mul.
 op [^] : (G_T, int) -> G_T as G_T_pow.
 
 op G_1_log : G_1 -> int.
+op G_2_log : G_2 -> int.
 op G_T_log : G_T -> int.
 
-op e : (G_1, G_1) -> G_T as G_1_pair.
+op e : (G_1, G_2) -> G_T as G_1_G_2_pair.
 
 (*
    From easycrypt ElGamal:
@@ -36,43 +43,60 @@ op e : (G_1, G_1) -> G_T as G_1_pair.
 op [%%] : (int,int) -> int as int_mod.
 
 axiom q_1_pos : 0 < q_1.
+axiom q_2_pos : 0 < q_2.
 axiom q_T_pos : 0 < q_T.
 
 axiom q_pos : 0 < q.
 
-(* Axioms largely pulled from ElGamal.  Note that G_1 and G_T have the same order if the order is prime. *)
+(* Axioms largely pulled from ElGamal.  Note that G_1, G_2, and G_T have the same order if the order is prime. *)
 
 axiom G_1_mult_1 : forall (x : G_1), x * g_1_i = x.
 axiom G_1_exp_0 : forall (x : G_1), x ^ 0 = g_1_i.
 axiom G_1_exp_S : forall (x : G_1, k : int), k > 0 => x ^ k = x * (x^(k-1)).
 
+axiom G_2_mult_1 : forall (x : G_2), x * g_2_i = x.
+axiom G_2_exp_0 : forall (x : G_2), x ^ 0 = g_2_i.
+axiom G_2_exp_S : forall (x : G_2, k : int), k > 0 => x ^ k = x * (x^(k-1)).
+
 axiom G_T_mult_1 : forall (x : G_T), x * g_T_i = x.
 axiom G_T_exp_0 : forall (x : G_T), x ^ 0 = g_T_i.
 axiom G_T_exp_S : forall (x : G_T, k : int), k > 0 => x ^ k = x * (x^(k-1)).
 
-axiom bilinearity : forall (x : G_1, y : G_1, a : int, b : int), e(x ^ a, y ^ b) = e(x, y) ^ (a * b).
-(* axiom non_degenerate : !(e(g_1, g_1) = g_T_i). *)
+axiom bilinearity : forall (x : G_1, y : G_2, a : int, b : int), e(x ^ a, y ^ b) = e(x, y) ^ (a * b).
+(* axiom non_degenerate : !(e(g_1, g_2) = g_T_i). *)
 
-axiom G_1_pow_add_1 :
+axiom G_2_pow_add_1 :
  forall (x, y:int), g_1 ^ (x + y) = g_1 ^ x * g_1 ^ y.
+
+axiom G_1_pow_add_2 :
+ forall (x, y:int), g_2 ^ (x + y) = g_2 ^ x * g_2 ^ y.
 
 axiom G_T_pow_add :
  forall (x, y:int), g_T ^ (x + y) = g_T ^ x * g_T ^ y.
 
-axiom G_1_pow_mult_1 :
+axiom G_2_pow_mult_1 :
  forall (x, y:int),  (g_1 ^ x) ^ y = g_1 ^ (x * y).
+
+axiom G_1_pow_mult_2 :
+ forall (x, y:int),  (g_2 ^ x) ^ y = g_2 ^ (x * y).
 
 axiom G_T_pow_mult :
  forall (x, y:int),  (g_T ^ x) ^ y = g_T ^ (x * y).
 
-axiom G_1_log_pow_1 :
- forall (g_1': G_1), g_1 ^ G_1_log(g_1') = g_1'.
+axiom G_2_log_pow_1 :
+ forall (g_1': G_2), g_1 ^ G_2_log(g_1') = g_1'.
+
+axiom G_1_log_pow_2 :
+ forall (g_2': G_1), g_2 ^ G_1_log(g_2') = g_2'.
 
 axiom G_T_log_pow :
  forall (g_T':G_T), g_T ^ G_T_log(g_T') = g_T'.
 
-axiom G_1_pow_mod_1 :
- forall (z:int), g_1 ^ (z%%q_1) = g_1 ^ z.
+axiom G_2_pow_mod_1 :
+ forall (z:int), g_1 ^ (z%%q_2) = g_1 ^ z.
+
+axiom G_1_pow_mod_2 :
+ forall (z:int), g_2 ^ (z%%q_1) = g_2 ^ z.
 
 axiom G_T_pow_mod :
  forall (z:int), g_T ^ (z%%q_T) = g_T ^ z.
@@ -91,17 +115,22 @@ axiom mod_bound :
 
 pop Rand_exp : () -> (int).
 pop Rand_G_1 : () -> (G_1).
+pop Rand_G_2 : () -> (G_2).
 
 (* axiom Rand_G_1_exp_def() : x = Rand_G_1_exp() ~ y = [0..q-1] : true ==> x = y. *)
-axiom Rand_G_1_def() : x = Rand_G_1() ~ y = Rand_exp() : true ==> x = g_1 ^ y.
+axiom Rand_G_1_def() : x = Rand_G_1() ~ y = Rand_exp() : true ==> x = g_2 ^ y.
 
-adversary Adv (adv_public_key_1 : G_1) : (message * G_1) {message -> G_1; (message) -> G_1}.
+axiom Rand_G_2_def() : x = Rand_G_2() ~ y = Rand_exp() : true ==> x = g_1 ^ y.
 
-game blsfull_EF = {
-  var sk : int
-  var pk : G_1
+adversary Adv (adv_public_key_1 : G_2, adv_public_key_2 : int) : (message * G_1) {message -> G_1; (message) -> G_1; (message) -> int}.
+
+game blsfullMODEL_EF = {
+  var sk1 : int
+  var pk1 : G_2
+  var var3 : int
   var queried : message list
   var count_Hash : int
+  var count_testFunction2 : int
   var count_Sign : int
   var count_Verify : int
   var rand_oracle : (message, G_1) map
@@ -115,36 +144,67 @@ game blsfull_EF = {
   }
 
   fun Sign(M : message) : G_1 = {
+    var sigsig : G_1;
+    var sig2 : G_1;
     var sig : G_1;
-    var preSig : G_1;
     var output : G_1;
+    var var27 : int;
     count_Sign = count_Sign + 1;
-    preSig = Hash(M);
-    sig = (preSig ^ sk);
-    output = sig;
+    sig = Hash(M);
+    sigsig = (sig ^ sk1);
+    sig2 = Hash(M);
+    var27 = testFunction3();
+    output = sigsig;
     queried = M :: queried;
     return output;
   }
 
-  abs A = Adv{Hash, Sign}
+  fun testFunction2(M : message) : int = {
+    var testVariable3 : G_1;
+    var output : int;
+    var hhh : G_1;
+    var hhh1 : G_1;
+    count_testFunction2 = count_testFunction2 + 1;
+    hhh = Hash(M);
+    hhh1 = (hhh ^ var3);
+    testVariable3 = (hhh1 ^ sk1);
+    output = var3;
+    return output;
+  }
+
+  abs A = Adv{Hash, Sign, testFunction2}
 
   fun Verify(M : message, sig : G_1) : bool = {
-    var output : bool;
     var h : G_1;
+    var output : bool;
+    var var4 : G_1;
     count_Verify = count_Verify + 1;
     h = Hash(M);
-    output = (e(h, pk) = e(sig, g_1));
+    if((e(h, pk1) = e(sig, g_1))) {
+      output = true;
+    }
+    else {
+      output = false;
+    }
+    output = (e(h, pk1) = e(sig, g_1));
+    var4 = (g_2 ^ var3);
     return output;
   }
 
   fun Init() : bool = {
+    var var5 : int;
+    var var333 : G_2;
     var x : int;
+    count_testFunction2 = 0;
     count_Hash = 0;
     count_Sign = 0;
     count_Verify = 0;
+    var333 = Rand_G_2();
     x = Rand_exp();
-    pk = (g_1 ^ x);
-    sk = x;
+    pk1 = (g_1 ^ x);
+    sk1 = x;
+    var3 = Rand_exp();
+    var5 = testFunction3();
     rand_oracle = empty_map;
     queried = [];
     return true;
@@ -157,7 +217,7 @@ game blsfull_EF = {
     var dummy : bool;
 
     dummy = Init();
-    (M, sig) = A(pk);
+    (M, sig) = A(pk1, var3);
 
     v = Verify(M, sig);
     return v && !mem(M, queried);
